save for now.

nobits_yunus.bpl
@@ -16,8 +16,8 @@ type String = [int]int;
 
 // return length of a string
 function length(string: String) returns(int);
-axiom(forall string: String :: length(string) >= 0);
-axiom(forall string: String :: string[length(string)] == 0);
+axiom(forall string: String :: {length(string)} length(string) >= 0);
+axiom(forall string: String :: {length(string)} string[length(string)] == 0);
 
 // compare two strings. return true if they are equal. Otherwise, return false.
 function cmpstr(str1: String, str2: String) returns(bool);
@@ -26,16 +26,18 @@ axiom(forall str1, str2: String :: !cmpstr(str1, str2) ==> ((length(str1) != len
 
 // count how many 'c' exists upto 'upper_limit' in 'string'
 function count(string: String, 	c: char, upper_limit: int) returns(int);
-axiom(forall string: String, c: char, i: int :: (i >= 0 && string[i]==c) ==> (count(string, c, i) == (1 + count(string, c, i-1))));
-axiom(forall string: String, c: char, i: int :: (i >= 0 && string[i]!=c) ==> (count(string, c, i) == count(string, c, i-1)));
+axiom(forall string: String, c: char, i: int :: count(string, c, i) >= 0);
 axiom(forall string: String, c: char, i: int :: (i < 0) ==> (count(string, c, i) == 0));
+axiom(forall string: String, c: char, i: int :: (i >= 0 && string[i]!=c) ==> (count(string, c, i) == count(string, c, i-1)));
+axiom(forall string: String, c: char, i: int :: (i >= 0 && string[i]==c) ==> (count(string, c, i) == (1 + count(string, c, i-1))));
+
+
 
 
 // summation of elements in array
 function summation(A: [int]int, i: int) returns(int);
 axiom(forall A: [int]int, i: int :: {summation(A, i-1)} summation(A, i) == (A[i] + summation(A, i-1)));
 axiom(forall A: [int]int, i: int :: (i < 0) ==> summation(A, i) == 0);
-
 
 var Cum: [int]int;
 var Tot: int;
@@ -51,14 +53,26 @@ procedure encodeAndDecode(string: String) returns(out: String);
 implementation encodeAndDecode(string: String) returns(out: String) {
 
   var lo,r0,r: int;
+	var lo_arr, r0_arr, r_arr: [int]int;
 	var i: int;
 	var x: int;
 	var c: char;
 	var len: int;
+	var deneme: String;
+
+  assume (forall j:int :: j >= 0 ==> (deneme[j] < 256 && deneme[j] >= 0));
+  assume (exists k:int :: (k >= 0 && deneme[k] == 0) && (forall j:int :: (k != j) ==> (deneme[j] != 0)));
+	assume (deneme[3] == 0);
 
 	len := length(string);
 	// Calculate static intervals
 
+	assert(len >= 0);
+	assert(string[len]==0);
+	assert(length(deneme) == 3);
+	assert(count(deneme, 0, length(deneme)) == 1);
+	assert(count(string, 0, len) >= 1);
+	
 	Cum[0] := 0;
 	i := 1;
 	while (i < 256)
@@ -72,31 +86,44 @@ implementation encodeAndDecode(string: String) returns(out: String) {
 	Tot := Cum[i - 1];
 
 	assert(Cum[0] == 0);
-	assert(forall k: int:: {Cum[k-1]} ((1 <= k) && (k < 256)) ==> (Cum[k] == Cum[k-1] + count(string, k, len-1)));
-	assert(Tot == Cum[255]); // TODO: assert(Tot == len)
+	assert(forall k: int:: {Cum[k-1]} ((1 <= k) && (k < 256)) ==> ((Cum[k] - Cum[k-1]) == count(string, k, len-1)));
+	assert(Tot == len);
 
 	
   // ENCODING PART
 	lo := 0;
 	r0 := 1;
 
-	r := r0;
+	r := 0;
 	while (r == 0)
 	{
 	  lo := 0;
 		r := r0;
 
+		r_arr[-1] := r;
+		lo_arr[-1] := lo;
+		
 		i := 0;
-		while (i < len) {
+		while (i < len)
+		invariant(i <= len);
+		invariant((i > 0) ==> ((lo == lo_arr[i-1]) && (r == r_arr[i-1])));
+		invariant(forall k: int :: {Cum[string[k]]} (0 <= k && k < i) ==> (r_arr[k] == (((r_arr[k-1] * Cum[string[k]]) / Tot) - ((r_arr[k-1] * Cum[string[k]-1]) / Tot))));  // TODO: without trigger hangs
+		invariant(forall k: int :: {Cum[string[k]]} (0 <= k && k < i) ==> (lo_arr[k] == (lo_arr[k-1] + ((r_arr[k-1] * Cum[string[k]]) / Tot))));  // TODO: without trigger hangs
+		{
 		  c := string[i];
-		  lo := lo + ((r * Cum[c-1]) / Tot);
-			r := ((r * Cum[c])/Tot) - ((r * Cum[c-1])/Tot);
+			
+		  lo_arr[i] := lo + ((r * Cum[c-1]) / Tot);
+			lo := lo_arr[i];
+
+			r_arr[i] := ((r * Cum[c])/Tot) - ((r * Cum[c-1])/Tot);
+			r := r_arr[i];
+			
+			i := i + 1;
 		}
 
 		r0 := r0 * 2;
 	}
 
-	assert(r != 0);
 
 	// DECODING PART
 	r := r0 / 2;
